
---

# Egyenletek

---

> 1. feladat
>
> $$
> \begin{aligned}
> 2[2(2x-1)-1]-1 = 0
> \end{aligned}
> $$

---

> 2. feladat
>
> $$
> \begin{aligned}
> 4[2(3x-4)-3]-4 = 0
> \end{aligned}
> $$

---

> 3. feladat
>
> $$
> \begin{aligned}
> 2{5[3(x-1)-4]-2} = 16
> \end{aligned}
> $$

---

> 4. feladat
>
> $$
> \begin{aligned}
> (2x+3)(x+4)*(x-1)(x+3) = 0
> \end{aligned}
> $$

---

> 5. feladat
>
> $$
> \begin{aligned}
> (4x-12)(x-11)*(3x-6)(x+8) = 0
> \end{aligned}
> $$

---

> 6. feladat
>
> $$
> \begin{aligned}
> 3(2x-7)-4(5-2x) = 3x+3
> \end{aligned}
> $$

---

> 7. feladat
>
> $$
> \begin{aligned}
> (1+x)(3x+4)-(2x+1)(x-3) = x(x-4)+2
> \end{aligned}
> $$

---

> 8. feladat
>
> $$
> \begin{aligned}
> \frac{2x-4}{3}+\frac{x-4}{2} = 2x
> \end{aligned}
> $$

---

> 9. feladat
>
> $$
> \begin{aligned}
> \frac{3x-7}{5}-\frac{x-7}{4}+\frac{3x+5}{2} = 1
> \end{aligned}
> $$

---

> 10. feladat
>
> $$
> \begin{aligned}
> \frac{x-4}{x+3}-\frac{x+2}{x+3} = 3
> \end{aligned}
> $$

---

> 11. feladat
>
> $$
> \begin{aligned}
> \frac{2x+3}{5}-\frac{x+2}{4} = \frac{x-3}{3}
> \end{aligned}
> $$

---

> 12. feladat
>
> $$
> \begin{aligned}
> \frac{2x}{3}-\frac{3x}{2} = \frac{1}{6}
> \end{aligned}
> $$

---